   \begin{subequations}
 \label{eq:BCs}
 	 \begin{align}
 	c_{s,t+s-1} + k_{s+1,t+s} &= (1-\tau_b)w_t (2-\ell_{s,t}^m - \ell_{s,t}^f) + r_{t+s-1}k_{s,t+s-1} & \forall t\text{ and for $s=1$} \\
 	c_{s,t+s-1} + k_{s+1,t+s} &= b_{t+s-1}^f+(1-\tau_b)w_t (1-\ell_{s,t}^m ) + r_{t+s-1}k_{s,t+s-1} & \forall t\text{ and for $s=2$} \\
 	c_{s,t+s-1} + k_{s+1,t+s} &= b_{t+s-1}^f+ b_{t+s-1}^m  + r_{t+s-1}k_{s,t+s-1} & \forall t\text{ and for $s=3$} \\
 	c_{s,t+s-1} + k_{s+1,t+s} &= b_{t+s-1}^f + r_{t+s-1}k_{s,t+s-1} & \forall t\text{ and for $s=4$} 
 \end{align}
 \end{subequations}
